Optimizations/Construction.thy
@@ -1,0 +1,781 @@
+section \<open>Graph Construction Phase\<close>
+
+theory
+  Construction
+imports
+  Proofs.Bisimulation
+  Proofs.IRGraphFrames
+begin
+
+lemma add_const_nodes:
+  assumes xn: "kind g x = (ConstantNode (IntVal b xv))"
+  assumes yn: "kind g y = (ConstantNode (IntVal b yv))"
+  assumes zn: "kind g z = (AddNode x y)"
+  assumes wn: "kind g w = (ConstantNode (intval_add (IntVal b xv) (IntVal b yv)))"
+  assumes val: "intval_add (IntVal b xv) (IntVal b yv) = IntVal b v1"
+  assumes ez: "g m \<turnstile> (kind g z) \<mapsto> (IntVal b v1)"
+  assumes ew: "g m \<turnstile> (kind g w) \<mapsto> (IntVal b v2)"
+  shows "v1 = v2"
+proof -
+  have zv: "g m \<turnstile> (kind g z) \<mapsto> IntVal b v1"
+    using eval.AddNode eval.ConstantNode xn yn zn val by metis
+  have wv: "g m \<turnstile> (kind g w) \<mapsto> IntVal b v2"
+    using eval.ConstantNode wn ew by blast 
+  show ?thesis using evalDet zv wv ew ez
+    using ConstantNode val wn by auto
+qed
+
+(* these are incorrect with the introduction of accurate addition semantics *)
+(* most obviously due to the resultant b being either 32 or 64 *)
+lemma add_val_xzero:
+  shows "intval_add (IntVal b 0) (IntVal b yv) = (IntVal b yv)"
+  unfolding intval_add.simps sorry
+
+lemma add_val_yzero:
+  shows "intval_add (IntVal b xv) (IntVal b 0) = (IntVal b xv)"
+  unfolding intval_add.simps sorry
+
+text_raw \<open>\Snip{CreateAddNode}%\<close>
+fun create_add :: "IRGraph \<Rightarrow> ID \<Rightarrow> ID \<Rightarrow> IRNode" where 
+  "create_add g x y = 
+    (case (kind g x) of 
+      ConstantNode (IntVal b xv) \<Rightarrow> 
+        (case (kind g y) of
+          ConstantNode (IntVal b yv) \<Rightarrow> 
+            ConstantNode (intval_add (IntVal b xv) (IntVal b yv)) | 
+          _ \<Rightarrow> if xv = 0 then RefNode y else AddNode x y
+        ) |
+      _ \<Rightarrow> (case (kind g y) of
+            ConstantNode (IntVal b yv) \<Rightarrow> 
+              if yv = 0 then RefNode x else AddNode x y |
+            _ \<Rightarrow> AddNode x y
+           )
+    )"
+text_raw \<open>\EndSnip\<close>
+
+
+text_raw \<open>\Snip{AddNodeCreate}%\<close>
+lemma add_node_create:
+  assumes xv: "g m \<turnstile> (kind g x) \<mapsto> IntVal b xv"
+  assumes yv: "g m \<turnstile> (kind g y) \<mapsto> IntVal b yv"
+  assumes res: "res = intval_add (IntVal b xv) (IntVal b yv)"
+  shows 
+    "(g m \<turnstile> (AddNode x y) \<mapsto> res) \<and>
+     (g m \<turnstile> (create_add g x y) \<mapsto> res)"
+text_raw \<open>\EndSnip\<close>
+proof -
+  let ?P = "(g m \<turnstile> (AddNode x y) \<mapsto> res)"
+  let ?Q = "(g m \<turnstile> (create_add g x y) \<mapsto> res)"
+  have P: ?P
+    using xv yv res eval.AddNode by blast
+  have Q: ?Q
+  proof (cases "is_ConstantNode (kind g x)")
+    case xconst: True
+    then show ?thesis
+    proof (cases "is_ConstantNode (kind g y)")
+      case yconst: True
+      have "create_add g x y = ConstantNode res"
+        using xconst yconst
+        using ConstantNodeE is_ConstantNode_def xv yv res by auto
+      then show ?thesis using eval.ConstantNode by simp
+    next
+      case ynotconst: False
+      have "kind g x = ConstantNode (IntVal b xv)"
+        using ConstantNodeE xconst
+        by (metis is_ConstantNode_def xv)
+      then have add_def:
+        "create_add g x y = (if xv = 0 then RefNode y else AddNode x y)"
+        using xconst ynotconst is_ConstantNode_def
+        unfolding create_add.simps
+        by (simp split: IRNode.split)
+      then show ?thesis
+      proof (cases "xv = 0")
+        case xzero: True
+        have ref: "create_add g x y = RefNode y"
+          using xzero add_def 
+          by meson
+        have refval: "g m \<turnstile> RefNode y \<mapsto> IntVal b yv"
+          using eval.RefNode yv by simp
+        have "res = IntVal b yv"
+          using res unfolding xzero add_val_xzero by simp
+        then show ?thesis using xzero ref refval by simp
+      next
+        case xnotzero: False
+        then show ?thesis
+          using P add_def by presburger
+      qed
+    qed
+next
+  case notxconst: False
+  then show ?thesis
+    proof (cases "is_ConstantNode (kind g y)")
+      case yconst: True
+      have "kind g y = ConstantNode (IntVal b yv)"
+        using ConstantNodeE yconst
+        by (metis is_ConstantNode_def yv)
+      then have add_def:
+        "create_add g x y = (if yv = 0 then RefNode x else AddNode x y)"
+        using notxconst yconst is_ConstantNode_def
+        unfolding create_add.simps
+        by (simp split: IRNode.split)
+      then show ?thesis
+      proof (cases "yv = 0")
+        case yzero: True
+        have ref: "create_add g x y = RefNode x"
+          using yzero add_def 
+          by meson
+        have refval: "g m \<turnstile> RefNode x \<mapsto> IntVal b xv"
+          using eval.RefNode xv by simp
+        have "res = IntVal b xv"
+          using res unfolding yzero add_val_yzero by simp
+        then show ?thesis using yzero ref refval by simp
+      next
+        case ynotzero: False
+        then show ?thesis
+          using P add_def by presburger
+      qed
+      
+    next
+      case notyconst: False
+      have "create_add g x y = AddNode x y"
+        using notxconst notyconst is_ConstantNode_def 
+        create_add.simps by (simp split: IRNode.split)
+      then show ?thesis
+        using P by presburger
+    qed
+qed
+  from P Q show ?thesis by simp
+qed
+
+(* The following function definition and lemmas designed to hide stamps
+   from the definition of if_node_create for the ITP paper which does
+   not include stamps *)
+fun add_node_fake :: "ID \<Rightarrow> IRNode \<Rightarrow> IRGraph \<Rightarrow> IRGraph" where
+  "add_node_fake nid k g = add_node nid (k, VoidStamp) g"
+lemma add_node_lookup_fake:
+  assumes "gup = add_node_fake nid k g"
+  assumes "nid \<notin> ids g"
+  shows "kind gup nid = k"
+  using add_node_lookup proof (cases "k = NoNode")
+  case True
+  have "kind g nid = NoNode"
+    using assms(2)
+    using not_in_g by blast
+  then show ?thesis using assms
+    by (metis add_node_fake.simps add_node_lookup)
+next
+  case False
+  then show ?thesis
+    by (simp add: add_node_lookup assms(1))
+qed
+lemma add_node_unchanged_fake:
+  assumes "new \<notin> ids g"
+  assumes "nid \<in> ids g"
+  assumes "gup = add_node_fake new k g"
+  assumes "wff_graph g"
+  shows "unchanged (eval_usages g nid) g gup"
+  using add_node_fake.simps add_node_unchanged assms by blast
+
+lemma dom_add_unchanged:
+  assumes "nid \<in> ids g"
+  assumes "g' = add_node_fake n k g"
+  assumes "nid \<noteq> n"
+  shows "nid \<in> ids g'"
+  using add_changed assms(1) assms(2) assms(3) by force
+
+lemma preserve_wff:
+  assumes wff: "wff_graph g"
+  assumes "nid \<notin> ids g"
+  assumes closed: "inputs g' nid \<union> succ g' nid \<subseteq> ids g"
+  assumes g': "g' = add_node_fake nid k g"
+  shows "wff_graph g'"
+  using assms unfolding wff_folds
+  apply (intro conjI)
+      apply (metis dom_add_unchanged)
+     apply (metis add_node_unchanged_fake assms(1) kind_unchanged)
+  sorry
+
+lemma equal_closure_bisimilar:
+  assumes "{P'. (g m h \<turnstile> nid \<leadsto> P')} = {P'. (g' m h \<turnstile> nid \<leadsto> P')}"
+  shows "nid . g \<sim> g'"
+  by (metis assms weak_bisimilar.simps mem_Collect_eq)
+
+lemma wff_size:
+  assumes "nid \<in> ids g"
+  assumes "wff_graph g"
+  assumes "isAbstractEndNodeType (kind g nid)"
+  shows "card (usages g nid) > 0"
+  using assms unfolding wff_folds
+  by fastforce
+
+lemma sequentials_have_successors:
+  assumes "is_sequential_node n"
+  shows "size (successors_of n) > 0"
+  using assms by (cases n; auto)
+
+lemma step_reaches_successors_only:
+  assumes "(g \<turnstile> (nid, m, h) \<rightarrow> (nid', m, h))"
+  assumes wff: "wff_graph g"
+  shows "nid' \<in> succ g nid \<or> nid' \<in> usages g nid"
+  using assms proof (induct "(nid, m, h)" "(nid', m, h)"rule: step.induct)
+  case SequentialNode
+  then show ?case using sequentials_have_successors
+    by (metis nth_mem succ.simps)
+next
+  case (IfNode cond tb fb val)
+  then show ?case using successors_of_IfNode
+    by (simp add: IfNode.hyps(1))
+next
+  case (EndNodes i phis inputs vs)
+  have "nid \<in> ids g"
+    using assms(1) step_in_ids
+    by blast
+  then have usage_size: "card (usages g nid) > 0"
+    using wff EndNodes(1) wff_size
+    by blast
+  then have usage_size: "size (sorted_list_of_set (usages g nid)) > 0"
+    by (metis length_sorted_list_of_set)
+  have "usages g nid \<subseteq> ids g"
+    using wff by fastforce
+  then have finite_usage: "finite (usages g nid)"
+    by (metis bot_nat_0.extremum_strict list.size(3) sorted_list_of_set.infinite usage_size)
+  from EndNodes(2) have "nid' \<in> usages g nid"
+    unfolding any_usage.simps
+    using usage_size finite_usage
+    by (metis hd_in_set length_greater_0_conv sorted_list_of_set(1))
+  then show ?case
+    by simp
+next
+  case RefNode
+  then show ?case using successors_of_RefNode
+    by simp
+next
+  case (NewInstanceNode f obj ref)
+  then show ?case using successors_of_NewInstanceNode by simp
+next
+  case (LoadFieldNode f obj ref v)
+  then show ?case by simp
+next
+  case (SignedDivNode x y zero sb v1 v2 v)
+  then show ?case by simp
+next
+  case (SignedRemNode x y zero sb v1 v2 v)
+  then show ?case by simp
+next
+  case (StaticLoadFieldNode f v)
+  then show ?case by simp
+next
+  case (StoreFieldNode f newval uu obj val ref)
+  then show ?case by simp
+next
+  case (StaticStoreFieldNode f newval uv val)
+  then show ?case by simp
+qed
+
+lemma stutter_closed:
+  assumes "g m h \<turnstile> nid \<leadsto> nid'"
+  assumes "wff_graph g"
+  shows "\<exists> n \<in> ids g . nid' \<in> succ g n \<or> nid' \<in> usages g n"
+  using assms
+proof (induct nid nid' rule: stutter.induct)
+  case (StutterStep nid nid')
+  have "nid \<in> ids g"
+    using StutterStep.hyps step_in_ids by blast
+  then show ?case using StutterStep step_reaches_successors_only
+    by blast
+next
+  case (Transitive nid nid'' nid')
+  then show ?case
+    by blast
+qed
+
+
+lemma unchanged_step:
+  assumes "g \<turnstile> (nid, m, h) \<rightarrow> (nid', m, h)"
+  assumes wff: "wff_graph g"
+  assumes kind: "kind g nid = kind g' nid"
+  assumes unchanged: "unchanged (eval_usages g nid) g g'"
+  assumes succ: "succ g nid = succ g' nid"
+  (*assumes usage: "unchanged (usages g nid) g g'"*)
+  shows "g' \<turnstile> (nid, m, h) \<rightarrow> (nid', m, h)"
+using assms proof (induct "(nid, m, h)" "(nid', m, h)" rule: step.induct)
+case SequentialNode
+  then show ?case
+    by (metis step.SequentialNode)
+next
+  case (IfNode cond tb fb val)
+  then show ?case using stay_same step.IfNode
+    by (metis (no_types, lifting) IRNodes.inputs_of_IfNode child_unchanged inputs.elims list.set_intros(1))
+next
+  case (EndNodes i phis inputs vs)
+  then show ?case sorry (* this is going to be a big problem *)
+next
+  case RefNode
+  then show ?case
+    using step.RefNode by presburger
+next
+  case (NewInstanceNode f obj ref)
+  then show ?case using step.NewInstanceNode
+    by metis
+next
+  case (LoadFieldNode f obj ref v)
+  have "obj \<in> inputs g nid"
+    using LoadFieldNode(1) inputs_of_LoadFieldNode 
+    using opt_to_list.simps
+    by (simp add: LoadFieldNode.hyps(1))
+  then have "unchanged (eval_usages g obj) g g'"
+    using unchanged
+    using child_unchanged by blast
+  then have "g' m \<turnstile> kind g' obj \<mapsto> ObjRef ref"
+    using unchanged wff stay_same
+    using LoadFieldNode.hyps(2) by presburger
+  then show ?case using step.LoadFieldNode
+    by (metis LoadFieldNode.hyps(1) LoadFieldNode.hyps(3) LoadFieldNode.hyps(4) assms(3))
+next
+  case (SignedDivNode x y zero sb v1 v2 v)
+  have "x \<in> inputs g nid"
+    using SignedDivNode(1) inputs_of_SignedDivNode
+    using opt_to_list.simps
+    by (simp add: SignedDivNode.hyps(1))
+  then have "unchanged (eval_usages g x) g g'"
+    using unchanged
+    using child_unchanged by blast
+  then have "g' m \<turnstile> kind g' x \<mapsto> v1"
+    using unchanged wff stay_same
+    using SignedDivNode.hyps(2) by presburger
+  have "y \<in> inputs g nid"
+    using SignedDivNode(1) inputs_of_SignedDivNode
+    using opt_to_list.simps
+    by (simp add: SignedDivNode.hyps(1))
+  then have "unchanged (eval_usages g y) g g'"
+    using unchanged
+    using child_unchanged by blast
+  then have "g' m \<turnstile> kind g' y \<mapsto> v2"
+    using unchanged wff stay_same
+    using SignedDivNode.hyps(3) by presburger
+  then show ?case using step.SignedDivNode
+    by (metis SignedDivNode.hyps(1) SignedDivNode.hyps(4) SignedDivNode.hyps(5) \<open>g' m \<turnstile> kind g' x \<mapsto> v1\<close> kind)
+next
+  case (SignedRemNode x y zero sb v1 v2 v)
+  have "x \<in> inputs g nid"
+    using SignedRemNode(1) inputs_of_SignedRemNode
+    using opt_to_list.simps
+    by (simp add: SignedRemNode.hyps(1))
+  then have "unchanged (eval_usages g x) g g'"
+    using unchanged
+    using child_unchanged by blast
+  then have "g' m \<turnstile> kind g' x \<mapsto> v1"
+    using unchanged wff stay_same
+    using SignedRemNode.hyps(2) by presburger
+  have "y \<in> inputs g nid"
+    using SignedRemNode(1) inputs_of_SignedRemNode
+    using opt_to_list.simps
+    by (simp add: SignedRemNode.hyps(1))
+  then have "unchanged (eval_usages g y) g g'"
+    using unchanged
+    using child_unchanged by blast
+  then have "g' m \<turnstile> kind g' y \<mapsto> v2"
+    using unchanged wff stay_same
+    using SignedRemNode.hyps(3) by presburger
+  then show ?case
+    by (metis SignedRemNode.hyps(1) SignedRemNode.hyps(4) SignedRemNode.hyps(5) \<open>g' m \<turnstile> kind g' x \<mapsto> v1\<close> kind step.SignedRemNode)
+next
+  case (StaticLoadFieldNode f v)
+  then show ?case using step.StaticLoadFieldNode
+    by metis
+next
+  case (StoreFieldNode f newval uu obj val ref)
+  have "obj \<in> inputs g nid"
+    using StoreFieldNode(1) inputs_of_StoreFieldNode
+    using opt_to_list.simps
+    by (simp add: StoreFieldNode.hyps(1))
+  then have "unchanged (eval_usages g obj) g g'"
+    using unchanged
+    using child_unchanged by blast
+  then have "g' m \<turnstile> kind g' obj \<mapsto> ObjRef ref"
+    using unchanged wff stay_same
+    using StoreFieldNode.hyps(3) by presburger
+  have "newval \<in> inputs g nid"
+    using StoreFieldNode(1) inputs_of_StoreFieldNode
+    using opt_to_list.simps
+    by (simp add: StoreFieldNode.hyps(1))
+  then have "unchanged (eval_usages g newval) g g'"
+    using unchanged
+    using child_unchanged by blast
+  then have "g' m \<turnstile> kind g' newval \<mapsto> val"
+    using unchanged wff stay_same
+    using StoreFieldNode.hyps(2) by blast
+  then show ?case using step.StoreFieldNode
+    by (metis StoreFieldNode.hyps(1) StoreFieldNode.hyps(4) StoreFieldNode.hyps(5) \<open>g' m \<turnstile> kind g' obj \<mapsto> ObjRef ref\<close> assms(3))
+next
+  case (StaticStoreFieldNode f newval uv val)
+  have "newval \<in> inputs g nid"
+    using StoreFieldNode(1) inputs_of_StoreFieldNode
+    using opt_to_list.simps
+    by (simp add: StaticStoreFieldNode.hyps(1))
+  then have "unchanged (eval_usages g newval) g g'"
+    using unchanged
+    using child_unchanged by blast
+  then have "g' m \<turnstile> kind g' newval \<mapsto> val"
+    using unchanged wff stay_same
+    using StaticStoreFieldNode.hyps(2) by blast
+  then show ?case using step.StaticStoreFieldNode
+    by (metis StaticStoreFieldNode.hyps(1) StaticStoreFieldNode.hyps(3) StaticStoreFieldNode.hyps(4) kind)
+qed
+
+
+lemma unchanged_closure:
+  assumes "nid \<notin> ids g"
+  assumes wff: "wff_graph g \<and> wff_graph g'"
+  assumes g': "g' = add_node_fake nid k g"
+  assumes "nid' \<in> ids g"
+  shows "(g m h \<turnstile> nid' \<leadsto> nid'') \<longleftrightarrow> (g' m h \<turnstile> nid' \<leadsto> nid'')" 
+    (is "?P \<longleftrightarrow> ?Q")
+proof
+  assume P: "?P"
+  have niddiff: "nid \<noteq> nid'"
+    using assms
+    by blast
+  from P show "?Q" using assms niddiff
+  proof (induction rule: stutter.induct)
+    case (StutterStep start e)
+    have unchanged: "unchanged (eval_usages g start) g g'"
+      using StutterStep.prems(4) add_node_unchanged_fake assms(1) g' wff by blast
+    have succ_same: "succ g start = succ g' start"
+      using StutterStep.prems(4) kind_unchanged succ.simps unchanged by presburger
+    have "kind g start = kind g' start"
+      by (metis StutterStep.prems(4) add_node_fake.elims add_node_unchanged assms(1) assms(2) g' kind_unchanged)
+    then have "g' \<turnstile> (start, m, h) \<rightarrow> (e, m, h)"
+      using unchanged_step wff unchanged succ_same
+      by (meson StutterStep.hyps)
+    then show ?case
+      using stutter.StutterStep by blast
+  next
+    case (Transitive nid nid'' nid')
+    then show ?case
+      by (metis add_node_unchanged_fake kind_unchanged step_in_ids stutter.Transitive stutter.cases succ.simps unchanged_step)
+  qed
+next
+  assume Q: "?Q"
+  have niddiff: "nid \<noteq> nid'"
+    using assms
+    by blast
+  from Q show "?P" using assms niddiff
+  proof (induction rule: stutter.induct)
+    case (StutterStep start e)
+    have "eval_usages g' start \<subseteq> eval_usages g start"
+      using g' eval_usages sorry
+    then have unchanged: "unchanged (eval_usages g' start) g' g"
+      by (smt (verit, ccfv_SIG) StutterStep.prems(4) add_node_unchanged_fake assms(1) g' subset_iff unchanged.simps wff)
+    have succ_same: "succ g start = succ g' start"
+      using StutterStep.prems(4) eval_usages_self node_unchanged succ.simps unchanged
+      by (metis (no_types, lifting) StutterStep.hyps step_in_ids)
+    have "kind g start = kind g' start"
+      by (metis StutterStep.prems(4) add_node_fake.elims add_node_unchanged assms(1) assms(2) g' kind_unchanged)
+    then have "g \<turnstile> (start, m, h) \<rightarrow> (e, m, h)"
+      using StutterStep(1) wff unchanged_step unchanged succ_same 
+      sorry (* :( *)
+    then show ?case
+      using stutter.StutterStep by blast
+  next
+    case (Transitive nid nid'' nid')
+    then show ?case
+      using add_node_unchanged_fake kind_unchanged step_in_ids stutter.Transitive stutter.cases succ.simps unchanged_step
+      sorry
+  qed
+qed
+
+text_raw \<open>\Snip{CreateIfNode}%\<close>
+fun create_if :: "IRGraph \<Rightarrow> ID \<Rightarrow> ID \<Rightarrow> ID \<Rightarrow> IRNode"
+  where 
+  "create_if g cond tb fb = 
+    (case (kind g cond) of 
+      ConstantNode condv \<Rightarrow> 
+        RefNode (if (val_to_bool condv) then tb else fb) |
+      _ \<Rightarrow> (if tb = fb then
+              RefNode tb
+            else 
+              IfNode cond tb fb)
+    )"
+text_raw \<open>\EndSnip\<close>
+
+
+lemma if_node_create_bisimulation:
+  fixes h :: FieldRefHeap
+  assumes wff: "wff_graph g"
+  assumes cv: "g m \<turnstile> (kind g cond) \<mapsto> cv"
+  assumes fresh: "nid \<notin> ids g"
+  assumes closed: "{cond, tb, fb} \<subseteq> ids g"
+  assumes gif: "gif = add_node_fake nid (IfNode cond tb fb) g"
+  assumes gcreate: "gcreate = add_node_fake nid (create_if g cond tb fb) g"
+
+  shows "nid . gif \<sim> gcreate"
+
+proof -
+  have indep: "\<not>(eval_uses g cond nid)"
+    using cv eval_in_ids fresh no_external_use wff by blast
+  have "kind gif nid = IfNode cond tb fb"
+    using gif add_node_lookup by simp
+  then have "{cond, tb, fb} = inputs gif nid \<union> succ gif nid"
+    using inputs_of_IfNode successors_of_IfNode
+    by (metis empty_set inputs.simps insert_is_Un list.simps(15) succ.simps)
+  then have wff_gif: "wff_graph gif"
+    using closed wff preserve_wff
+    using fresh gif by presburger
+  have "create_if g cond tb fb = IfNode cond tb fb \<or>
+        create_if g cond tb fb = RefNode tb \<or>
+        create_if g cond tb fb = RefNode fb"
+    by (cases "kind g cond"; auto)
+  then have "kind gcreate nid  = IfNode cond tb fb \<or>
+        kind gcreate nid = RefNode tb \<or>
+        kind gcreate nid = RefNode fb" 
+    using gcreate add_node_lookup
+    using add_node_lookup_fake fresh by presburger
+  then have "inputs gcreate nid \<union> succ gcreate nid \<subseteq> {cond, tb, fb}"
+    using inputs_of_IfNode successors_of_IfNode inputs_of_RefNode successors_of_RefNode
+    by force
+  then have wff_gcreate: "wff_graph gcreate"
+    using closed wff preserve_wff fresh gcreate
+    by (metis subset_trans)
+  have tb_unchanged: "{nid'. (gif m h \<turnstile> tb \<leadsto> nid')} = {nid'. (gcreate m h \<turnstile> tb \<leadsto> nid')}"
+  proof -
+    have "\<not>(\<exists>n \<in> ids g. nid \<in> succ g n \<or> nid \<in> usages g n)"
+      using wff
+      by (metis (no_types, lifting) fresh mem_Collect_eq subsetD usages.simps wff_folds(1,3))
+    then have "nid \<notin> {nid'. (g m h \<turnstile> tb \<leadsto> nid')}"
+      using wff stutter_closed
+      by (metis mem_Collect_eq)
+    have gif_set: "{nid'. (gif m h \<turnstile> tb \<leadsto> nid')} = {nid'. (g m h \<turnstile> tb \<leadsto> nid')}"
+      using unchanged_closure fresh wff gif closed wff_gif
+      by blast
+    have gcreate_set: "{nid'. (gcreate m h \<turnstile> tb \<leadsto> nid')} = {nid'. (g m h \<turnstile> tb \<leadsto> nid')}"
+      using unchanged_closure fresh wff gcreate closed wff_gcreate
+      by blast
+    from gif_set gcreate_set show ?thesis by simp
+  qed
+  have fb_unchanged: "{nid'. (gif m h \<turnstile> fb \<leadsto> nid')} = {nid'. (gcreate m h \<turnstile> fb \<leadsto> nid')}"
+      proof -
+    have "\<not>(\<exists>n \<in> ids g. nid \<in> succ g n \<or> nid \<in> usages g n)"
+      using wff
+      by (metis (no_types, lifting) fresh mem_Collect_eq subsetD usages.simps wff_folds(1,3))
+    then have "nid \<notin> {nid'. (g m h \<turnstile> fb \<leadsto> nid')}"
+      using wff stutter_closed
+      by (metis mem_Collect_eq)
+    have gif_set: "{nid'. (gif m h \<turnstile> fb \<leadsto> nid')} = {nid'. (g m h \<turnstile> fb \<leadsto> nid')}"
+      using unchanged_closure fresh wff gif closed wff_gif
+      by blast
+    have gcreate_set: "{nid'. (gcreate m h \<turnstile> fb \<leadsto> nid')} = {nid'. (g m h \<turnstile> fb \<leadsto> nid')}"
+      using unchanged_closure fresh wff gcreate closed wff_gcreate
+      by blast
+    from gif_set gcreate_set show ?thesis by simp
+  qed
+  show ?thesis
+proof (cases "\<exists> val . (kind g cond) = ConstantNode val")
+  let ?gif_closure = "{P'. (gif m h \<turnstile> nid \<leadsto> P')}"
+  let ?gcreate_closure = "{P'. (gcreate m h \<turnstile> nid \<leadsto> P')}"
+  case constantCond: True
+  obtain val where val: "(kind g cond) = ConstantNode val"
+    using constantCond by blast
+  then show ?thesis 
+  proof (cases "val_to_bool val")
+    case constantTrue: True
+    have if_kind: "kind gif nid = (IfNode cond tb fb)"
+      using gif add_node_lookup by simp
+    have if_cv: "gif m \<turnstile> (kind gif cond) \<mapsto> val"
+      by (metis ConstantNodeE add_node_unchanged_fake cv eval_in_ids fresh gif stay_same val wff)
+    have "(gif \<turnstile> (nid, m, h) \<rightarrow> (tb, m, h))"
+      using step.IfNode if_kind if_cv
+      using constantTrue by presburger
+    then have gif_closure: "?gif_closure = {tb} \<union> {nid'. (gif m h \<turnstile> tb \<leadsto> nid')}"
+      using stuttering_successor by presburger 
+    have ref_kind: "kind gcreate nid = (RefNode tb)"
+      using gcreate add_node_lookup constantTrue constantCond unfolding create_if.simps
+      by (simp add: val)
+    have "(gcreate \<turnstile> (nid, m, h) \<rightarrow> (tb, m, h))"
+      using step.RefNode ref_kind by simp
+    then have gcreate_closure: "?gcreate_closure = {tb} \<union> {nid'. (gcreate m h \<turnstile> tb \<leadsto> nid')}"
+      using stuttering_successor
+      by auto
+    from gif_closure gcreate_closure have "?gif_closure = ?gcreate_closure"
+      using tb_unchanged by simp
+    then show ?thesis
+      using equal_closure_bisimilar by simp
+  next
+    case constantFalse: False
+    have if_kind: "kind gif nid = (IfNode cond tb fb)"
+      using gif add_node_lookup by simp
+    have if_cv: "gif m \<turnstile> (kind gif cond) \<mapsto> val"
+      by (metis ConstantNodeE add_node_unchanged_fake cv eval_in_ids fresh gif stay_same val wff)
+    have "(gif \<turnstile> (nid, m, h) \<rightarrow> (fb, m, h))"
+      using step.IfNode if_kind if_cv
+      using constantFalse by presburger
+    then have gif_closure: "?gif_closure = {fb} \<union> {nid'. (gif m h \<turnstile> fb \<leadsto> nid')}"
+      using stuttering_successor by presburger
+    have ref_kind: "kind gcreate nid = RefNode fb"
+      using add_node_lookup_fake constantFalse fresh gcreate val by force
+    then have "(gcreate \<turnstile> (nid, m, h) \<rightarrow> (fb, m, h))"
+      using step.RefNode by presburger
+    then have gcreate_closure: "?gcreate_closure = {fb} \<union> {nid'. (gcreate m h \<turnstile> fb \<leadsto> nid')}"
+      using stuttering_successor by presburger
+    from gif_closure gcreate_closure have "?gif_closure = ?gcreate_closure"
+      using fb_unchanged by simp
+    then show ?thesis
+      using equal_closure_bisimilar by simp
+  qed
+next
+  let ?gif_closure = "{P'. (gif m h \<turnstile> nid \<leadsto> P')}"
+  let ?gcreate_closure = "{P'. (gcreate m h \<turnstile> nid \<leadsto> P')}"
+  case notConstantCond: False
+  then show ?thesis 
+  proof (cases "tb = fb")
+    case equalBranches: True
+     have if_kind: "kind gif nid = (IfNode cond tb fb)"
+      using gif add_node_lookup by simp
+    have "(gif \<turnstile> (nid, m, h) \<rightarrow> (tb, m, h)) \<or> (gif \<turnstile> (nid, m, h) \<rightarrow> (fb, m, h))"
+      using step.IfNode if_kind cv apply (cases "val_to_bool cv")
+      apply (metis add_node_fake.simps add_node_unchanged eval_in_ids fresh gif stay_same wff)
+      by (metis add_node_unchanged_fake eval_in_ids fresh gif stay_same wff)
+    then have gif_closure: "?gif_closure = {tb} \<union> {nid'. (gif m h \<turnstile> tb \<leadsto> nid')}"
+      using equalBranches
+      using stuttering_successor by presburger
+    have iref_kind: "kind gcreate nid = (RefNode tb)"
+      using gcreate add_node_lookup notConstantCond equalBranches
+      unfolding create_if.simps
+      by (cases "(kind g cond)"; auto)
+    then have "(gcreate \<turnstile> (nid, m, h) \<rightarrow> (tb, m, h))"
+      using step.RefNode by simp
+    then have gcreate_closure: "?gcreate_closure = {tb} \<union> {nid'. (gcreate m h \<turnstile> tb \<leadsto> nid')}"
+      using stuttering_successor by presburger
+    from gif_closure gcreate_closure have "?gif_closure = ?gcreate_closure"
+      using tb_unchanged by simp
+    then show ?thesis
+      using equal_closure_bisimilar by simp
+  next
+    case uniqueBranches: False
+    let ?tb_closure = "{tb} \<union> {nid'. (gif m h \<turnstile> tb \<leadsto> nid')}"
+    let ?fb_closure = "{fb} \<union> {nid'. (gif m h \<turnstile> fb \<leadsto> nid')}"
+     have if_kind: "kind gif nid = (IfNode cond tb fb)"
+      using gif add_node_lookup by simp
+    have if_step: "(gif \<turnstile> (nid, m, h) \<rightarrow> (tb, m, h)) \<or> (gif \<turnstile> (nid, m, h) \<rightarrow> (fb, m, h))"
+      using step.IfNode if_kind cv apply (cases "val_to_bool cv")
+      apply (metis add_node_fake.simps add_node_unchanged eval_in_ids fresh gif stay_same wff)
+      by (metis add_node_unchanged_fake eval_in_ids fresh gif stay_same wff)
+    then have gif_closure: "?gif_closure = ?tb_closure \<or> ?gif_closure = ?fb_closure"
+      using stuttering_successor by presburger
+    have gc_kind: "kind gcreate nid = (IfNode cond tb fb)"
+      using gcreate add_node_lookup notConstantCond uniqueBranches
+      unfolding create_if.simps
+      by (cases "(kind g cond)"; auto)
+    then have "(gcreate \<turnstile> (nid, m, h) \<rightarrow> (tb, m, h)) \<or> (gcreate \<turnstile> (nid, m, h) \<rightarrow> (fb, m, h))"
+      by (metis add_node_lookup_fake fresh gcreate gif if_step)
+    then have gcreate_closure: "?gcreate_closure = ?tb_closure \<or> ?gcreate_closure = ?fb_closure"
+      by (metis add_node_lookup_fake fresh gc_kind gcreate gif gif_closure)
+    from gif_closure gcreate_closure have "?gif_closure = ?gcreate_closure"
+      using tb_unchanged fb_unchanged
+      by (metis add_node_lookup_fake fresh gc_kind gcreate gif)
+    then show ?thesis
+      using equal_closure_bisimilar by simp
+  qed
+qed
+qed
+
+
+text_raw \<open>\Snip{IfNodeCreate}%\<close>
+lemma if_node_create:
+  assumes wff: "wff_graph g"
+  assumes cv: "g m \<turnstile> (kind g cond) \<mapsto> cv"
+  assumes fresh: "nid \<notin> ids g"
+  assumes gif: "gif = add_node_fake nid (IfNode cond tb fb) g"
+  assumes gcreate: "gcreate = add_node_fake nid (create_if g cond tb fb) g"
+  shows "\<exists>nid'. (gif m h \<turnstile> nid \<leadsto> nid') \<and> (gcreate m h \<turnstile> nid \<leadsto> nid')"
+text_raw \<open>\EndSnip\<close>
+proof (cases "\<exists> val . (kind g cond) = ConstantNode val")
+  case True
+  show ?thesis
+  proof -
+    obtain val where val: "(kind g cond) = ConstantNode val"
+      using True by blast
+    have cond_exists: "cond \<in> ids g"
+      using cv eval_in_ids by auto
+    have if_kind: "kind gif nid = (IfNode cond tb fb)"
+      using gif add_node_lookup by simp
+    have if_cv: "gif m \<turnstile> (kind gif cond) \<mapsto> val"
+      using step.IfNode if_kind
+      using True eval.ConstantNode gif fresh
+      using stay_same cond_exists
+      using val
+      using add_node.rep_eq kind.rep_eq by auto
+    have if_step: "gif \<turnstile> (nid,m,h) \<rightarrow> (if val_to_bool val then tb else fb,m,h)"
+    proof -
+      show ?thesis using step.IfNode if_kind if_cv 
+        by (simp)
+    qed
+    have create_step: "gcreate \<turnstile> (nid,m,h) \<rightarrow> (if val_to_bool val then tb else fb,m,h)"
+    proof -
+      have create_kind: "kind gcreate nid = (create_if g cond tb fb)"
+        using gcreate add_node_lookup_fake
+        using fresh by blast
+      have create_fun: "create_if g cond tb fb = RefNode (if val_to_bool val then tb else fb)"
+        using True create_kind val by simp 
+      show ?thesis using step.RefNode create_kind create_fun if_cv 
+        by (simp)
+    qed
+    then show ?thesis using StutterStep create_step if_step
+      by blast
+  qed
+next
+  case not_const: False
+  obtain nid' where "nid' = (if val_to_bool cv then tb else fb)"
+    by blast
+  have nid_eq: "(gif \<turnstile> (nid,m,h) \<rightarrow> (nid',m,h)) \<and> (gcreate \<turnstile> (nid,m,h) \<rightarrow> (nid',m,h))"
+  proof -
+    have indep: "\<not>(eval_uses g cond nid)"
+      using no_external_use
+      using cv eval_in_ids fresh wff by blast
+    have nid': "nid' = (if val_to_bool cv then tb else fb)"
+      by (simp add: \<open>nid' = (if val_to_bool cv then tb else fb)\<close>)
+    have gif_kind: "kind gif nid = (IfNode cond tb fb)"
+      using add_node_lookup_fake gif
+      using fresh by blast
+    then have "nid \<noteq> cond"
+      using cv fresh indep
+      using eval_in_ids by blast
+    have "unchanged (eval_usages g cond) g gif"
+      using gif add_node_unchanged_fake
+      using cv eval_in_ids fresh wff by blast
+    then obtain cv2 where cv2: "gif m \<turnstile> (kind gif cond) \<mapsto> cv2" 
+      using cv gif wff stay_same by blast
+    then have "cv = cv2"
+      using indep gif cv
+      using \<open>nid \<noteq> cond\<close>
+      using fresh
+      using \<open>unchanged (eval_usages g cond) g gif\<close> evalDet stay_same wff by blast
+    then have eval_gif: "(gif \<turnstile> (nid,m,h) \<rightarrow> (nid',m,h))"
+      using step.IfNode gif_kind nid' cv2 
+      by auto
+    have gcreate_kind: "kind gcreate nid = (create_if g cond tb fb)"
+      using gcreate add_node_lookup_fake
+      using fresh by blast
+    have eval_gcreate: "gcreate \<turnstile> (nid,m,h) \<rightarrow> (nid',m,h)"
+    proof (cases "tb = fb")
+      case True
+      have "create_if g cond tb fb = RefNode tb"
+        using not_const True by (cases "(kind g cond)"; auto)
+      then show ?thesis
+        using True gcreate_kind nid' step.RefNode
+        by (simp)
+    next
+      case False
+      have "create_if g cond tb fb = IfNode cond tb fb"
+        using not_const False by (cases "(kind g cond)"; auto)
+      then show ?thesis
+        using eval_gif gcreate gif
+        using IfNode \<open>cv = cv2\<close> cv2 gif_kind nid' by auto
+    qed
+    show ?thesis
+      using eval_gcreate eval_gif StutterStep by blast
+  qed
+  show ?thesis using nid_eq StutterStep by meson
+qed
+
+end
