Proofs/Bisimulation.thy
@@ -1,0 +1,42 @@
+section \<open>Proof Infrastructure\<close>
+subsection \<open>Bisimulation\<close>
+
+theory Bisimulation
+imports
+  Stuttering
+begin
+
+(* WIP strong bisimilar
+fun strongly_bisimilar :: "
+(IRGraph \<times> ID \<times> MapState \<times> FieldRefHeap) rel
+\<Rightarrow> (IRGraph \<times> ID \<times> MapState \<times> FieldRefHeap)
+\<Rightarrow> (IRGraph \<times> ID \<times> MapState \<times> FieldRefHeap)
+\<Rightarrow> bool"
+  where
+  "strongly_bisimilar \<R> (g1, nid1, m1, h1) (g2, nid2, m2, h2) =
+    ((((g1, nid1, m1, h1), (g2, nid2, m2, h2)) \<in> \<R>) \<longrightarrow>
+    ((\<forall>P'. (g1 \<turnstile> (nid1, m1, h1) \<rightarrow> P') \<longrightarrow> (\<exists>Q' . (g2 \<turnstile> (nid2, m2, h2) \<rightarrow> Q') \<and> ((g1,P'), (g2,Q')) \<in> \<R>)) \<and>
+    (\<forall>Q'. (g2 \<turnstile> (nid2, m2, h2) \<rightarrow> Q') \<longrightarrow> (\<exists>P' . (g1 \<turnstile> (nid1, m1, h1) \<rightarrow> P') \<and> ((g1,P'), (g2,Q')) \<in> \<R>))))"
+*)
+
+inductive weak_bisimilar :: "ID \<Rightarrow> IRGraph \<Rightarrow> IRGraph \<Rightarrow> bool"
+  ("_ . _ \<sim> _") for nid where
+  "\<lbrakk>\<forall>P'. (g m h \<turnstile> nid \<leadsto> P') \<longrightarrow> (\<exists>Q' . (g' m h \<turnstile> nid \<leadsto> Q') \<and> P' = Q');
+    \<forall>Q'. (g' m h \<turnstile> nid \<leadsto> Q') \<longrightarrow> (\<exists>P' . (g m h \<turnstile> nid \<leadsto> P') \<and> P' = Q')\<rbrakk>
+  \<Longrightarrow> nid . g \<sim> g'"
+
+text \<open>A strong bisimilution between no-op transitions\<close>
+inductive strong_noop_bisimilar :: "ID \<Rightarrow> IRGraph \<Rightarrow> IRGraph \<Rightarrow> bool"
+  ("_ | _ \<sim> _") for nid where
+  "\<lbrakk>\<forall>P'. (g \<turnstile> (nid, m, h) \<rightarrow> P') \<longrightarrow> (\<exists>Q' . (g' \<turnstile> (nid, m, h) \<rightarrow> Q') \<and> P' = Q');
+    \<forall>Q'. (g' \<turnstile> (nid, m, h) \<rightarrow> Q') \<longrightarrow> (\<exists>P' . (g \<turnstile> (nid, m, h) \<rightarrow> P') \<and> P' = Q')\<rbrakk>
+  \<Longrightarrow> nid | g \<sim> g'"
+
+lemma lockstep_strong_bisimilulation:
+  assumes "g' = replace_node nid node g"
+  assumes "g \<turnstile> (nid, m, h) \<rightarrow> (nid', m, h)"
+  assumes "g' \<turnstile> (nid, m, h) \<rightarrow> (nid', m, h)"
+  shows "nid | g \<sim> g'"
+  using assms(2) assms(3) stepDet strong_noop_bisimilar.simps by blast
+
+end
