Proofs/Form.thy
@@ -1,0 +1,57 @@
+subsection \<open>Formedness Properties\<close>
+
+theory Form
+imports
+  Semantics.IREval
+begin
+
+definition wff_start where
+  "wff_start g = (0 \<in> ids g \<and>
+    is_StartNode (kind g 0))"
+
+definition wff_closed where
+  "wff_closed g = 
+    (\<forall> n \<in> ids g .
+      inputs g n \<subseteq> ids g \<and>
+      succ g n \<subseteq> ids g \<and>
+      kind g n \<noteq> NoNode)"
+
+definition wff_phis where
+  "wff_phis g = 
+    (\<forall> n \<in> ids g.
+      isPhiNodeType (kind g n) \<longrightarrow>
+      length (ir_values (kind g n))
+       = length (ir_ends 
+           (kind g (ir_merge (kind g n)))))"
+
+definition wff_ends where
+  "wff_ends g = 
+    (\<forall> n \<in> ids g .
+      isAbstractEndNodeType (kind g n) \<longrightarrow>
+      card (usages g n) > 0)"
+
+text_raw \<open>\Snip{wff_graph}%\<close>
+fun wff_graph :: "IRGraph \<Rightarrow> bool" where
+  "wff_graph g = (wff_start g \<and> wff_closed g \<and> wff_phis g \<and> wff_ends g)"
+text_raw \<open>\EndSnip\<close>
+
+lemmas wff_folds =
+  wff_graph.simps
+  wff_start_def
+  wff_closed_def
+  wff_phis_def
+  wff_ends_def
+
+fun wff_stamps :: "IRGraph \<Rightarrow> bool" where
+  "wff_stamps g = (\<forall> n \<in> ids g . 
+    (\<forall> v m . (g m \<turnstile> (kind g n) \<mapsto> v) \<longrightarrow> valid_value (stamp g n) v))"
+
+
+
+lemma wff_empty: "wff_graph start_end_graph"
+  unfolding start_end_graph_def wff_folds by simp
+
+lemma wff_eg2_sq: "wff_graph eg2_sq"
+  unfolding eg2_sq_def wff_folds by simp
+
+end
