Proofs/Rewrites.thy
@@ -1,0 +1,188 @@
+subsection \<open>Graph Rewriting\<close>
+
+theory
+  Rewrites
+imports
+  IRGraphFrames
+  Stuttering
+begin
+
+fun replace_usages :: "ID \<Rightarrow> ID \<Rightarrow> IRGraph \<Rightarrow> IRGraph" where
+  "replace_usages nid nid' g = replace_node nid (RefNode nid', stamp g nid') g"
+
+lemma replace_usages_effect:
+  assumes "g' = replace_usages nid nid' g"
+  shows "kind g' nid = RefNode nid'"
+  using assms replace_node_lookup replace_usages.simps IRNode.distinct(2069)
+  by (metis)
+
+lemma replace_usages_changeonly:
+  assumes "nid \<in> ids g"
+  assumes "g' = replace_usages nid nid' g"
+  shows "changeonly {nid} g g'"
+  using assms unfolding replace_usages.simps
+  by (metis DiffI changeonly.elims(3) ids_some replace_node_unchanged)
+
+lemma replace_usages_unchanged:
+  assumes "nid \<in> ids g"
+  assumes "g' = replace_usages nid nid' g"
+  shows "unchanged (ids g - {nid}) g g'"
+  using assms unfolding replace_usages.simps
+  by (smt (verit, del_insts) DiffE ids_some replace_node_unchanged unchanged.simps)
+
+
+
+fun nextNid :: "IRGraph \<Rightarrow> ID" where
+  "nextNid g = (Max (ids g)) + 1"
+
+lemma max_plus_one:
+  fixes c :: "ID set"
+  shows "\<lbrakk>finite c; c \<noteq> {}\<rbrakk> \<Longrightarrow> (Max c) + 1 \<notin> c"
+  by (meson Max_gr_iff less_add_one less_irrefl)
+
+lemma ids_finite:
+  "finite (ids g)"
+  by simp
+
+lemma nextNidNotIn:
+  "ids g \<noteq> {} \<longrightarrow> nextNid g \<notin> ids g"
+  unfolding nextNid.simps
+  using ids_finite max_plus_one by blast
+
+fun constantCondition :: "bool \<Rightarrow> ID \<Rightarrow> IRNode \<Rightarrow> IRGraph \<Rightarrow> IRGraph" where
+  "constantCondition val nid (IfNode cond t f) g = 
+    replace_node nid (IfNode (nextNid g) t f, stamp g nid) 
+      (add_node (nextNid g) ((ConstantNode (bool_to_val val)), default_stamp) g)" |
+  "constantCondition cond nid _ g = g"
+
+lemma constantConditionTrue:
+  assumes "kind g ifcond = IfNode cond t f"
+  assumes "g' = constantCondition True ifcond (kind g ifcond) g"
+  shows "g' \<turnstile> (ifcond, m, h) \<rightarrow> (t, m, h)"
+proof -
+  have if': "kind g' ifcond = IfNode (nextNid g) t f"
+    by (metis IRNode.simps(989) assms(1) assms(2) constantCondition.simps(1) replace_node_lookup)
+  have "bool_to_val True = (IntVal 1 1)"
+    by auto
+  have "ifcond \<noteq> (nextNid g)"
+    by (metis IRNode.simps(989) assms(1) emptyE ids_some nextNidNotIn)
+  then have c': "kind g' (nextNid g) = ConstantNode (IntVal 1 1)"
+    using assms(2) replace_node_unchanged
+    by (metis DiffI IRNode.distinct(585) \<open>bool_to_val True = IntVal 1 1\<close> add_node_lookup assms(1) constantCondition.simps(1) emptyE insertE not_in_g)
+  from if' c' show ?thesis using IfNode
+    by (smt (z3) ConstantNode val_to_bool.simps(1))
+qed
+
+lemma constantConditionFalse:
+  assumes "kind g ifcond = IfNode cond t f"
+  assumes "g' = constantCondition False ifcond (kind g ifcond) g"
+  shows "g' \<turnstile> (ifcond, m, h) \<rightarrow> (f, m, h)"
+proof -
+  have if': "kind g' ifcond = IfNode (nextNid g) t f"
+    by (metis IRNode.simps(989) assms(1) assms(2) constantCondition.simps(1) replace_node_lookup)
+  have "bool_to_val False = (IntVal 1 0)"
+    by auto
+  have "ifcond \<noteq> (nextNid g)"
+    by (metis IRNode.simps(989) assms(1) emptyE ids_some nextNidNotIn)
+  then have c': "kind g' (nextNid g) = ConstantNode (IntVal 1 0)"
+    using assms(2) replace_node_unchanged
+    by (metis DiffI IRNode.distinct(585) \<open>bool_to_val False = IntVal 1 0\<close> add_node_lookup assms(1) constantCondition.simps(1) emptyE insertE not_in_g)
+  from if' c' show ?thesis using IfNode
+    by (smt (z3) ConstantNode val_to_bool.simps(1))
+qed
+
+lemma diff_forall:
+  assumes "\<forall>n\<in>ids g - {nid}. cond n"
+  shows "\<forall>n. n \<in> ids g \<and> n \<notin> {nid} \<longrightarrow> cond n"
+  by (meson Diff_iff assms)
+
+lemma replace_node_changeonly:
+  assumes "g' = replace_node nid node g"
+  shows "changeonly {nid} g g'"
+  using assms replace_node_unchanged
+  unfolding changeonly.simps using diff_forall
+  sorry (* Isabelle isn't doing good *)
+
+lemma add_node_changeonly:
+  assumes "g' = add_node nid node g"
+  shows "changeonly {nid} g g'"
+  by (metis Rep_IRGraph_inverse add_node.rep_eq assms replace_node.rep_eq replace_node_changeonly)
+
+lemma constantConditionNoEffect:
+  assumes "\<not>(is_IfNode (kind g nid))"
+  shows "g = constantCondition b nid (kind g nid) g"
+  using assms apply (cases "kind g nid")
+  using constantCondition.simps 
+  apply presburger+
+  apply (metis is_IfNode_def)
+  using constantCondition.simps 
+  by presburger+
+
+lemma constantConditionIfNode:
+  assumes "kind g nid = IfNode cond t f"
+  shows "constantCondition val nid (kind g nid) g = 
+    replace_node nid (IfNode (nextNid g) t f, stamp g nid) 
+     (add_node (nextNid g) ((ConstantNode (bool_to_val val)), default_stamp) g)"
+  using constantCondition.simps
+  by (simp add: assms)
+
+lemma constantCondition_changeonly:
+  assumes "nid \<in> ids g"
+  assumes "g' = constantCondition b nid (kind g nid) g"
+  shows "changeonly {nid} g g'"
+proof (cases "is_IfNode (kind g nid)")
+  case True
+  have "nextNid g \<notin> ids g"
+    using nextNidNotIn by (metis emptyE)
+  then show ?thesis using assms
+    using replace_node_changeonly add_node_changeonly unfolding changeonly.simps
+    using True constantCondition.simps(1) is_IfNode_def
+    by (metis (full_types) DiffD2 Diff_insert_absorb)
+next
+  case False
+  have "g = g'"
+    using constantConditionNoEffect
+    using False assms(2) by blast
+  then show ?thesis by simp
+qed
+  
+
+lemma constantConditionNoIf:
+  assumes "\<forall>cond t f. kind g ifcond \<noteq> IfNode cond t f"
+  assumes "g' = constantCondition val ifcond (kind g ifcond) g"
+  shows "\<exists>nid' .(g m h \<turnstile> ifcond \<leadsto> nid') \<longleftrightarrow> (g' m h \<turnstile> ifcond \<leadsto> nid')"
+proof -
+  have "g' = g"
+    using assms(2) assms(1)
+    using constantConditionNoEffect
+    by (metis IRNode.collapse(11))
+  then show ?thesis by simp
+qed
+
+lemma constantConditionValid:
+  assumes "kind g ifcond = IfNode cond t f"
+  assumes "g m \<turnstile> kind g cond \<mapsto> v"
+  assumes "const = val_to_bool v"
+  assumes "g' = constantCondition const ifcond (kind g ifcond) g"
+  shows "\<exists>nid' .(g m h \<turnstile> ifcond \<leadsto> nid') \<longleftrightarrow> (g' m h \<turnstile> ifcond \<leadsto> nid')"
+proof (cases "const")
+  case True
+  have ifstep: "g \<turnstile> (ifcond, m, h) \<rightarrow> (t, m, h)"
+    by (meson IfNode True assms(1) assms(2) assms(3))
+  have ifstep': "g' \<turnstile> (ifcond, m, h) \<rightarrow> (t, m, h)"
+    using constantConditionTrue
+    using True assms(1) assms(4) by presburger
+  from ifstep ifstep' show ?thesis
+    using StutterStep by blast
+next
+  case False
+  have ifstep: "g \<turnstile> (ifcond, m, h) \<rightarrow> (f, m, h)"
+    by (meson IfNode False assms(1) assms(2) assms(3))
+  have ifstep': "g' \<turnstile> (ifcond, m, h) \<rightarrow> (f, m, h)"
+    using constantConditionFalse
+    using False assms(1) assms(4) by presburger
+  from ifstep ifstep' show ?thesis
+    using StutterStep by blast
+qed
+
+end
