Proofs/Stuttering.thy
@@ -1,3 +1,5 @@
+subsection \<open>Stuttering\<close>
+
 theory Stuttering
   imports
     Semantics.IRStepObj
@@ -14,5 +16,20 @@ inductive stutter:: "IRGraph \<Rightarrow> MapState \<Rightarrow> FieldRefHeap \
   "\<lbrakk>g \<turnstile> (nid,m,h) \<rightarrow> (nid'',m,h);
     g m h \<turnstile> nid'' \<leadsto> nid'\<rbrakk>
    \<Longrightarrow> g m h \<turnstile> nid \<leadsto> nid'"
+
+lemma stuttering_successor:
+  assumes "(g \<turnstile> (nid, m, h) \<rightarrow> (nid', m, h))"
+  shows "{P'. (g m h \<turnstile> nid \<leadsto> P')} = {nid'} \<union> {nid''. (g m h \<turnstile> nid' \<leadsto> nid'')}"
+proof -
+  have nextin: "nid' \<in> {P'. (g m h \<turnstile> nid \<leadsto> P')}"
+    using assms StutterStep by blast
+  have nextsubset: "{nid''. (g m h \<turnstile> nid' \<leadsto> nid'')} \<subseteq> {P'. (g m h \<turnstile> nid \<leadsto> P')}"
+    by (metis Collect_mono assms stutter.Transitive)
+  have "\<forall>n \<in> {P'. (g m h \<turnstile> nid \<leadsto> P')} . n = nid' \<or> n \<in> {nid''. (g m h \<turnstile> nid' \<leadsto> nid'')}"
+    using stepDet
+    by (metis (no_types, lifting) Pair_inject assms mem_Collect_eq stutter.simps)
+  then show ?thesis
+    using insert_absorb mk_disjoint_insert nextin nextsubset by auto
+qed
 
 end
